KZG_hiding.thy
@@ -37,19 +37,18 @@ type_synonym ('a', 'e')  adversary =
   "'a' commit \<Rightarrow> ('e' eval_position \<times> 'e' eval_value \<times> 'a' eval_witness) list \<Rightarrow> 
  'e' polynomial spmf"
 
-definition hiding_game :: "'e eval_position list \<Rightarrow> 'e polynomial \<Rightarrow> ('a, 'e) adversary \<Rightarrow> bool spmf"
-  where "hiding_game eval_pos \<phi> \<A> = TRY do {
-  _ :: unit \<leftarrow> assert_spmf (length eval_pos = max_deg \<and> distinct eval_pos);
+definition hiding_game :: "'e eval_position list \<Rightarrow> 'e polynomial \<Rightarrow> ('a, 'e) adversary \<Rightarrow> 'e polynomial spmf"
+  where "hiding_game eval_pos \<phi> \<A> = do {
   PK \<leftarrow> key_gen;
   let C = Commit PK \<phi>;
   let witn_tupel = map (\<lambda>i. (i, poly \<phi> i, createWitness PK \<phi> i)) eval_pos;
   \<phi>' \<leftarrow> \<A> C witn_tupel;
-  return_spmf (\<phi> = \<phi>')} ELSE return_spmf False"
+  return_spmf \<phi>'}"
 
 text \<open>put C and eval_poses in parameter and assert\<close>
 
 definition hiding_advantage :: "'e eval_position list \<Rightarrow>  'e polynomial \<Rightarrow> ('a, 'e) adversary \<Rightarrow> real"
-  where "hiding_advantage eval_pos \<phi> \<A> \<equiv> spmf (hiding_game eval_pos \<phi> \<A>) True"
+  where "hiding_advantage eval_pos \<phi> \<A> \<equiv> spmf (hiding_game eval_pos \<phi> \<A>) \<phi>"
 
 subsection \<open>DL game\<close>
 
@@ -69,11 +68,42 @@ lemma split_sample_distinct_coordinates_uniform_into_points:
   unfolding sample_distinct_coordinates_uniform_def 
   by (smt (verit) bind_return_spmf bind_spmf_cong map_spmf_bind_spmf pair_spmf_alt_def return_bind_spmf)
 
-definition sample_coords :: "('e mod_ring \<times> 'e mod_ring) list spmf"
+definition sample_n_coords :: "nat \<Rightarrow> ('e mod_ring \<times> 'e mod_ring) list spmf"
 where 
-  "sample_coords =
+  "sample_n_coords n =
     map_spmf (map (\<lambda>(x,y). (of_int_mod_ring (int x),of_int_mod_ring (int y))))
-    (sample_distinct_coordinates_uniform max_deg (order G\<^sub>p))"
+    (sample_distinct_coordinates_uniform n (order G\<^sub>p))"
+
+lemma length_pair_lists: "length xs = n \<Longrightarrow> length ys = n \<Longrightarrow> length (pair_lists (xs,ys)) = n"
+  by (induction "(xs,ys)" arbitrary: n xs ys rule: pair_lists.induct)simp+
+
+lemma sample_n_coords_length: "\<forall>xs \<in> set_spmf (sample_n_coords n). length xs \<le> n"
+proof -
+  have "length ` set_spmf (sample_n_coords n) = {n}"
+  proof -
+    have "length ` set_spmf (sample_n_coords n) = (length \<circ> (map (\<lambda>(x, y). (of_int_mod_ring (int x), of_int_mod_ring (int y)))) \<circ> pair_lists) ` ({xs. length xs = n \<and> distinct xs \<and> set xs \<subseteq> {..<order G\<^sub>p}} \<times> {xs. set xs \<subseteq> {..<order G\<^sub>p} \<and> length xs = n})"
+     unfolding sample_n_coords_def 
+    using set_spmf_sample_distinct_coordinates_uniform_list
+    by (simp add: image_comp)
+  also have "(length \<circ> (map (\<lambda>(x, y). (of_int_mod_ring (int x), of_int_mod_ring (int y)))) \<circ> pair_lists) ` ({xs. length xs = n \<and> distinct xs \<and> set xs \<subseteq> {..<order G\<^sub>p}} \<times> {xs. set xs \<subseteq> {..<order G\<^sub>p} \<and> length xs = n})
+    = (length \<circ> pair_lists) ` ({xs. length xs = n \<and> distinct xs \<and> set xs \<subseteq> {..<order G\<^sub>p}} \<times> {xs. set xs \<subseteq> {..<order G\<^sub>p} \<and> length xs = n})"
+    using length_map by simp
+  also have "(length \<circ> pair_lists) ` ({xs. length xs = n \<and> distinct xs \<and> set xs \<subseteq> {..<order G\<^sub>p}} \<times> {xs. set xs \<subseteq> {..<order G\<^sub>p} \<and> length xs = n}) = {n}"
+  proof -
+    have "length `{xs. length xs = n \<and> distinct xs \<and> set xs \<subseteq> {..<order G\<^sub>p}} = {n}"
+      sorry
+    moreover have "length `{xs. set xs \<subseteq> {..<order G\<^sub>p} \<and> length xs = n} = {n}"
+      sorry
+    ultimately show ?thesis using length_pair_lists sorry
+  qed
+  then show?thesis sorry
+  qed
+  then show ?thesis by fast
+qed
+    
+lemma sample_n_coords_dist: "\<forall>xs \<in> set_spmf (sample_n_coords n). distinct (map fst xs)"
+  sorry
+  
 
 
 lemma eval_on_lagrange_basis: "poly (lagrange_interpolation_poly xs_ys) x \<equiv> (let 
@@ -159,7 +189,7 @@ proof -
   proof -
     have "degree (lagrange_interpolation_poly xs_ys) \<le> max_deg"
       by (meson assms(2) degree_lagrange_interpolation_poly le_diff_conv le_trans nat_le_iff_add)
-    then show "\<^bold>g ^\<^bsub>G\<^sub>p\<^esub> poly (lagrange_interpolation_poly xs_ys) \<alpha> =  Commit 
+    then show "\<^bold>g ^\<^bsub>G\<^sub>p\<^esub> poly (lagrange_interpolation_poly xs_ys) \<alpha> = Commit 
     (map (\<lambda>t. \<^bold>g ^\<^bsub>G\<^sub>p\<^esub> \<alpha> ^ t) [0..<max_deg + 1]) (lagrange_interpolation_poly xs_ys)"
     unfolding Commit_def 
     using g_pow_PK_Prod_correct by presburger
@@ -167,32 +197,187 @@ proof -
   finally show ?thesis by fast
 qed
 
+lemma split_pow_div_G\<^sub>p[simp]: 
+  assumes "x\<noteq>0"
+  shows " \<^bold>g ^\<^bsub>G\<^sub>p\<^esub> (y/x) = (\<^bold>g ^\<^bsub>G\<^sub>p\<^esub> y) ^\<^bsub>G\<^sub>p\<^esub> (1/x)"
+  by (metis assms mod_ring_pow_pow_G\<^sub>p mult_cancel_left2 times_divide_eq_right)
+
+lemma witness_calc_correct: 
+  assumes dist: "distinct (map fst xs_ys)"
+  and length_xs_ys: "length xs_ys \<le> max_deg"
+  and \<alpha>_nin_xs: "\<alpha> \<notin> set (map fst xs_ys)"
+  shows "map (\<lambda>i. (i, poly (lagrange_interpolation_poly xs_ys) i, createWitness (map (\<lambda>t. \<^bold>g ^\<^bsub>G\<^sub>p\<^esub> \<alpha> ^ t) [0..<max_deg + 1]) (lagrange_interpolation_poly xs_ys) i)) (map fst xs_ys)
+    =  map (\<lambda>(x,y). (x,y,( \<^bold>g\<^bsub>G\<^sub>p\<^esub> ^\<^bsub>G\<^sub>p\<^esub> (poly (lagrange_interpolation_poly xs_ys) \<alpha>)  \<div>\<^bsub>G\<^sub>p\<^esub> \<^bold>g\<^bsub>G\<^sub>p\<^esub> ^\<^bsub>G\<^sub>p\<^esub> y) ^\<^bsub>G\<^sub>p\<^esub> (1/(\<alpha>-x)))) xs_ys"
+proof -
+  have "?thesis = (map (\<lambda>i. (fst i, poly (lagrange_interpolation_poly xs_ys) (fst i), createWitness (map (\<lambda>t. \<^bold>g ^\<^bsub>G\<^sub>p\<^esub> \<alpha> ^ t) [0..<max_deg + 1]) (lagrange_interpolation_poly xs_ys) (fst i))) xs_ys
+  =  map (\<lambda>(x,y). (x,y,( \<^bold>g\<^bsub>G\<^sub>p\<^esub> ^\<^bsub>G\<^sub>p\<^esub> (poly (lagrange_interpolation_poly xs_ys) \<alpha>)  \<div>\<^bsub>G\<^sub>p\<^esub> \<^bold>g\<^bsub>G\<^sub>p\<^esub> ^\<^bsub>G\<^sub>p\<^esub> y) ^\<^bsub>G\<^sub>p\<^esub> (1/(\<alpha>-x)))) xs_ys)"
+    by simp
+  also have "\<dots>"
+  proof(rule map_ext)
+    fix x
+    show "x \<in> set xs_ys \<longrightarrow>
+         (fst x, poly (lagrange_interpolation_poly xs_ys) (fst x),
+          createWitness (map (\<lambda>t. \<^bold>g ^\<^bsub>G\<^sub>p\<^esub> \<alpha> ^ t) [0..<max_deg + 1]) (lagrange_interpolation_poly xs_ys) (fst x)) =
+         (\<lambda>(x, y). (x, y, (\<^bold>g ^\<^bsub>G\<^sub>p\<^esub> (poly (lagrange_interpolation_poly xs_ys) \<alpha>) \<div>\<^bsub>G\<^sub>p\<^esub> \<^bold>g\<^bsub>G\<^sub>p\<^esub> ^\<^bsub>G\<^sub>p\<^esub> y) ^\<^bsub>G\<^sub>p\<^esub> (1 / (\<alpha> - x)))) x"
+    proof 
+      assume asm: "x \<in> set xs_ys"
+      then obtain xj yj where xj_yj: "(xj,yj) = x"
+        using prod.collapse by blast
+      moreover have "(xj, poly (lagrange_interpolation_poly xs_ys) xj, createWitness (map (\<lambda>t. \<^bold>g ^\<^bsub>G\<^sub>p\<^esub> \<alpha> ^ t) [0..<max_deg + 1]) (lagrange_interpolation_poly xs_ys) xj) 
+                   = (xj, yj, (\<^bold>g ^\<^bsub>G\<^sub>p\<^esub> (poly (lagrange_interpolation_poly xs_ys) \<alpha>) \<div>\<^bsub>G\<^sub>p\<^esub> \<^bold>g\<^bsub>G\<^sub>p\<^esub> ^\<^bsub>G\<^sub>p\<^esub> yj) ^\<^bsub>G\<^sub>p\<^esub> (1 / (\<alpha> - xj)))"
+      proof -
+        have \<alpha>_neg_xj: "\<alpha> \<noteq> xj"
+              by (metis asm assms(1) assms(3) entries_keysD entries_of_alist fst_eqD keys_of_alist xj_yj)
+
+        have "createWitness (map (\<lambda>t. \<^bold>g ^\<^bsub>G\<^sub>p\<^esub> \<alpha> ^ t) [0..<max_deg + 1]) (lagrange_interpolation_poly xs_ys) xj = (\<^bold>g ^\<^bsub>G\<^sub>p\<^esub> (poly (lagrange_interpolation_poly xs_ys) \<alpha>) \<div>\<^bsub>G\<^sub>p\<^esub> \<^bold>g\<^bsub>G\<^sub>p\<^esub> ^\<^bsub>G\<^sub>p\<^esub> yj) ^\<^bsub>G\<^sub>p\<^esub> (1 / (\<alpha> - xj))"
+          (is "?lhs = ?rhs")
+        proof -
+          have "?lhs = \<^bold>g ^\<^bsub>G\<^sub>p\<^esub> (poly (\<psi>_of (lagrange_interpolation_poly xs_ys) xj) \<alpha>)"
+            unfolding createWitness.simps Let_def 
+            using g_pow_PK_Prod_correct
+            by (meson assms(2) degree_lagrange_interpolation_poly degree_q_le_\<phi> diff_le_self le_trans)
+          also have "\<dots> = \<^bold>g ^\<^bsub>G\<^sub>p\<^esub> ((poly (lagrange_interpolation_poly xs_ys) \<alpha> - poly (lagrange_interpolation_poly xs_ys) xj)/(\<alpha>-xj))"
+              using \<alpha>_neg_xj \<phi>x_m_\<phi>u_eq_xmu_\<psi>x by simp
+          also have "\<dots> =  \<^bold>g ^\<^bsub>G\<^sub>p\<^esub> ((poly (lagrange_interpolation_poly xs_ys) \<alpha> - yj)/(\<alpha>-xj))"
+            using asm dist lagrange_interpolation_poly xj_yj by blast
+          also have "\<dots> =  (\<^bold>g ^\<^bsub>G\<^sub>p\<^esub> (poly (lagrange_interpolation_poly xs_ys) \<alpha> - yj)) ^\<^bsub>G\<^sub>p\<^esub> (1 / (\<alpha> - xj))"
+            using \<alpha>_neg_xj by force
+          also have "\<dots> = ?rhs"
+            using mod_ring_pow_mult_inv_G\<^sub>p by presburger
+          finally show ?thesis .
+        qed
+        then show ?thesis
+          using asm assms calculation lagrange_interpolation_poly by blast
+      qed
+      ultimately show "(fst x, poly (lagrange_interpolation_poly xs_ys) (fst x),
+          createWitness (map (\<lambda>t. \<^bold>g ^\<^bsub>G\<^sub>p\<^esub> \<alpha> ^ t) [0..<max_deg + 1]) (lagrange_interpolation_poly xs_ys) (fst x)) =
+         (\<lambda>(x, y). (x, y, (\<^bold>g ^\<^bsub>G\<^sub>p\<^esub> (poly (lagrange_interpolation_poly xs_ys) \<alpha>) \<otimes> inv (\<^bold>g ^\<^bsub>G\<^sub>p\<^esub> y)) ^\<^bsub>G\<^sub>p\<^esub> (1 / (\<alpha> - x)))) x"
+        by force
+    qed
+  qed
+  finally show ?thesis
+    by fast
+qed
+
+
 fun reduction
   :: "('a, 'e) adversary \<Rightarrow> ('a,'e) DL.adversary"                     
 where
   "reduction \<A> g_pow_a = do {
-    coords \<leftarrow> sample_coords;
-    let exp_coords = (0,g_pow_a)#map (\<lambda>(x,y). (x,\<^bold>g\<^bsub>G\<^sub>p\<^esub> ^\<^bsub>G\<^sub>p\<^esub> y)) coords;
+    coords \<leftarrow> sample_n_coords (max_deg); 
+    let exp_coords = (fst (hd coords),g_pow_a)#map (\<lambda>(x,y). (x,\<^bold>g\<^bsub>G\<^sub>p\<^esub> ^\<^bsub>G\<^sub>p\<^esub> y)) (tl coords);
     (\<alpha>, PK) \<leftarrow> Setup;
     let g_pow_\<phi>_of_\<alpha> = compute_g_pow_\<phi>_of_\<alpha> exp_coords \<alpha>;
-    let wtn_tuples = map (\<lambda>(x,y). (x,y,(g_pow_\<phi>_of_\<alpha>  \<div>\<^bsub>G\<^sub>p\<^esub> \<^bold>g\<^bsub>G\<^sub>p\<^esub> ^\<^bsub>G\<^sub>p\<^esub> y) ^\<^bsub>G\<^sub>p\<^esub> (1/\<alpha>-x))) coords;
+    let wtn_tuples = map (\<lambda>(x,y). (x,y,(g_pow_\<phi>_of_\<alpha>  \<div>\<^bsub>G\<^sub>p\<^esub> \<^bold>g\<^bsub>G\<^sub>p\<^esub> ^\<^bsub>G\<^sub>p\<^esub> y) ^\<^bsub>G\<^sub>p\<^esub> (1/(\<alpha>-x)))) (tl coords);
     \<phi>' \<leftarrow> \<A> g_pow_\<phi>_of_\<alpha> wtn_tuples;
-    _::unit \<leftarrow> assert_spmf (True); \<comment>\<open>\<phi>'= \<phi> coords (exp?)\<close>
     return_spmf (poly \<phi>' 0)}"
+
+(*sample n coords max_deg + 1 (for point (x,a) ) *)
 
 subsection \<open>Reduction proof\<close>
 
 subsubsection \<open>helping lemmas\<close>
 
+lemma helping_lemma_1:
+  assumes dist: "distinct (map fst (coords))"
+  and length_coords: "length coords \<le> max_deg"
+  shows
+"compute_g_pow_\<phi>_of_\<alpha> ((fst (hd coords),\<^bold>g ^\<^bsub>G\<^sub>p\<^esub> a)#map (\<lambda>(x,y). (x,\<^bold>g\<^bsub>G\<^sub>p\<^esub> ^\<^bsub>G\<^sub>p\<^esub> y)) (tl coords)) \<alpha>
+  = Commit (map (\<lambda>t. \<^bold>g\<^bsub>G\<^sub>p\<^esub> ^\<^bsub>G\<^sub>p\<^esub> (\<alpha>^t)) [0..<max_deg+1]) (lagrange_interpolation_poly ((fst (hd coords),a)#tl coords))"
+proof -
+  obtain xs_ys where xs_ys: "xs_ys = (fst (hd coords),a)#tl coords" by simp
+  have dist_xs_ys: "distinct (map fst xs_ys)"
+    using xs_ys dist
+    by (metis (no_types, lifting) distinct_singleton fst_conv list.collapse list.sel(2) list.simps(8) list.simps(9))
+  have length_xs_ys: "length xs_ys \<le> max_deg"
+    using assms(2) d_pos xs_ys by auto
+  show ?thesis 
+    using compute_g_pow_\<phi>_of_\<alpha>_is_Commit[OF dist_xs_ys length_xs_ys]
+    unfolding xs_ys by force
+qed
+  
 
 subsubsection \<open>reduction proof\<close>
 
 theorem
-  assumes "\<And>\<phi>. spmf (hiding_game eval_pos \<phi> \<A>) True = 1"
+  assumes "\<And>\<phi> eval_pos. length eval_pos \<le> max_deg \<and> distinct eval_pos \<longrightarrow> spmf (hiding_game eval_pos \<phi> \<A>) \<phi> = 1"
   shows "spmf (DL_G\<^sub>p.game (reduction \<A>)) True = 1"
+proof -
+   note [simp] = Let_def split_def
+
+  text \<open>abbreviations for the mod_ring version of sample uniform nat 
+  and the public key\<close>
+  let ?mr = "\<lambda>\<alpha>. (of_int_mod_ring (int \<alpha>)::'e mod_ring)"
+  let ?PK = "\<lambda>\<alpha>. (map (\<lambda>t. \<^bold>g\<^bsub>G\<^sub>p\<^esub> ^\<^bsub>G\<^sub>p\<^esub> ((?mr \<alpha>)^t)) [0..<max_deg+1])"
+
+  have "DL_G\<^sub>p.game (reduction \<A>) = TRY do { 
+    a \<leftarrow> sample_uniform (Coset.order G\<^sub>p);
+    a' \<leftarrow> reduction \<A> (\<^bold>g ^\<^bsub>G\<^sub>p\<^esub> (?mr a));
+    return_spmf (?mr a = a') 
+  } ELSE return_spmf False"
+    unfolding DL_G\<^sub>p.game_def by force
+  also have "\<dots> = TRY do { 
+    a \<leftarrow> sample_uniform (Coset.order G\<^sub>p);
+    a' \<leftarrow>  do {
+    coords \<leftarrow> sample_n_coords (max_deg);
+    let exp_coords = (fst (hd coords),(\<^bold>g ^\<^bsub>G\<^sub>p\<^esub> (?mr a)))#map (\<lambda>(x,y). (x,\<^bold>g\<^bsub>G\<^sub>p\<^esub> ^\<^bsub>G\<^sub>p\<^esub> y)) (tl coords);
+    (\<alpha>, PK) \<leftarrow> Setup;
+    let g_pow_\<phi>_of_\<alpha> = compute_g_pow_\<phi>_of_\<alpha> exp_coords \<alpha>;
+    let wtn_tuples = map (\<lambda>(x,y). (x,y,(g_pow_\<phi>_of_\<alpha>  \<div>\<^bsub>G\<^sub>p\<^esub> \<^bold>g\<^bsub>G\<^sub>p\<^esub> ^\<^bsub>G\<^sub>p\<^esub> y) ^\<^bsub>G\<^sub>p\<^esub> (1/(\<alpha>-x)))) (tl coords);
+    \<phi>' \<leftarrow> \<A> g_pow_\<phi>_of_\<alpha> wtn_tuples;
+    return_spmf (poly \<phi>' 0)};
+    return_spmf (of_int_mod_ring (int a) = a') 
+  } ELSE return_spmf False"
+    unfolding reduction.simps by fast
+  also have "\<dots> = TRY do { 
+    a \<leftarrow> sample_uniform (Coset.order G\<^sub>p);
+    coords \<leftarrow> sample_n_coords (max_deg);
+    \<phi>' \<leftarrow> do {
+    let exp_coords = (fst (hd coords),(\<^bold>g ^\<^bsub>G\<^sub>p\<^esub> (?mr a)))#map (\<lambda>(x,y). (x,\<^bold>g\<^bsub>G\<^sub>p\<^esub> ^\<^bsub>G\<^sub>p\<^esub> y)) (tl coords);
+    (\<alpha>, PK) \<leftarrow> Setup;
+    let g_pow_\<phi>_of_\<alpha> = compute_g_pow_\<phi>_of_\<alpha> exp_coords \<alpha>;
+    let wtn_tuples = map (\<lambda>(x,y). (x,y,(g_pow_\<phi>_of_\<alpha>  \<div>\<^bsub>G\<^sub>p\<^esub> \<^bold>g\<^bsub>G\<^sub>p\<^esub> ^\<^bsub>G\<^sub>p\<^esub> y) ^\<^bsub>G\<^sub>p\<^esub> (1/(\<alpha>-x)))) (tl coords);
+    \<phi>' \<leftarrow> \<A> g_pow_\<phi>_of_\<alpha> wtn_tuples;
+    return_spmf \<phi>'};
+    let a' = (poly \<phi>' 0);
+    return_spmf (of_int_mod_ring (int a) = a') 
+  } ELSE return_spmf False"
+    by force
+  also have "\<dots> = TRY do { 
+    a \<leftarrow> sample_uniform (Coset.order G\<^sub>p);
+    coords \<leftarrow> sample_n_coords (max_deg);
+    \<phi>' \<leftarrow> do {
+    let exp_coords = (fst (hd coords),(\<^bold>g ^\<^bsub>G\<^sub>p\<^esub> (?mr a)))#map (\<lambda>(x,y). (x,\<^bold>g\<^bsub>G\<^sub>p\<^esub> ^\<^bsub>G\<^sub>p\<^esub> y)) (tl coords);
+    \<alpha> :: nat \<leftarrow> sample_uniform (order G\<^sub>p);
+    let g_pow_\<phi>_of_\<alpha> = compute_g_pow_\<phi>_of_\<alpha> exp_coords (?mr \<alpha>);
+    let wtn_tuples = map (\<lambda>(x,y). (x,y,(g_pow_\<phi>_of_\<alpha>  \<div>\<^bsub>G\<^sub>p\<^esub> \<^bold>g\<^bsub>G\<^sub>p\<^esub> ^\<^bsub>G\<^sub>p\<^esub> y) ^\<^bsub>G\<^sub>p\<^esub> (1/((?mr \<alpha>)-x)))) (tl coords);
+    \<phi>' \<leftarrow> \<A> g_pow_\<phi>_of_\<alpha> wtn_tuples;
+    return_spmf \<phi>'};
+    let a' = (poly \<phi>' 0);
+    return_spmf (of_int_mod_ring (int a) = a') 
+  } ELSE return_spmf False"
+    unfolding Setup_def by force
+  also have "\<dots> = TRY do { 
+    a \<leftarrow> sample_uniform (Coset.order G\<^sub>p);
+    coords \<leftarrow> sample_n_coords (max_deg);
+    \<phi>' \<leftarrow> do {
+    let exp_coords = (fst (hd coords),(\<^bold>g ^\<^bsub>G\<^sub>p\<^esub> (?mr a)))#map (\<lambda>(x,y). (x,\<^bold>g\<^bsub>G\<^sub>p\<^esub> ^\<^bsub>G\<^sub>p\<^esub> y)) (tl coords);
+    \<alpha> :: nat \<leftarrow> sample_uniform (order G\<^sub>p);
+    let g_pow_\<phi>_of_\<alpha> = Commit (?PK \<alpha>) (lagrange_interpolation_poly ((fst (hd coords),?mr a)#tl coords));
+    let wtn_tuples = map (\<lambda>(x,y). (x,y,(g_pow_\<phi>_of_\<alpha>  \<div>\<^bsub>G\<^sub>p\<^esub> \<^bold>g\<^bsub>G\<^sub>p\<^esub> ^\<^bsub>G\<^sub>p\<^esub> y) ^\<^bsub>G\<^sub>p\<^esub> (1/((?mr \<alpha>)-x)))) (tl coords);
+    \<phi>' \<leftarrow> \<A> g_pow_\<phi>_of_\<alpha> wtn_tuples;
+    return_spmf \<phi>'};
+    let a' = (poly \<phi>' 0);
+    return_spmf (of_int_mod_ring (int a) = a') 
+  } ELSE return_spmf False"
+    using helping_lemma_1 sample_n_coords_length sample_n_coords_dist sorry
+  
+
+  show ?thesis
   using assms unfolding DL_G\<^sub>p.game_def hiding_game_def reduction.simps
   key_gen_def Let_def Setup_def
   sorry
+qed
 
 end
 
